Add clock to FBOS

CE_FBOS.v
@@ -2,142 +2,195 @@ Require Export CE_Aux.
 
 Import ListNotations.
 
+Import Lia.
+
 Definition set_second {A B C : Type} (p : A * B * C) (b : B) : A * B * C :=
 match p with
 | (a, b0, c) => (a, b, c)
 end.
 
-Fixpoint eval_fbos_expr (env : Environment) (id : nat) (exp : Expression) (eff : SideEffectList) :
-  nat * (Value + Exception) * SideEffectList :=
-match exp with
- | ENil => (id, inl VNil, eff)
- | ELit l => (id, inl (VLit l), eff)
- | EVar v => (id, get_value env (inl v), eff)
- | EFunId f => (id, get_value env (inr f), eff)
- | EFun vl e => (S id, inl (VClos env [] id vl e), eff)
- | ECons hd tl =>
-   match eval_fbos_expr env id hd eff with
-   | (id', inl hdv, eff') =>
-     match eval_fbos_expr env id' tl eff' with
-     | (id'', inl tlv, eff'') => (id'', inl (VCons hdv tlv), eff'')
-     | (id'', inr ex , eff'') => (id'', inr ex, eff'')
-     end
-   | (id', inr ex , eff') => (id', inr ex, eff')
-   end
- | ETuple l => let res := 
-           (fix eval_list env id exps eff : nat * ((list Value) + Exception) * SideEffectList := 
-               match exps with
-               | []    => (id, inl [], eff)
-               | x::xs => match eval_fbos_expr env id x eff with
-                          | (id', inl v , eff') => 
-                            let res := eval_list env id' xs eff' in
-                              match res with
-                              | (id'', inl xs', eff'') => (id'', inl (v::xs'), eff'')
-                              | (id'', inr ex , eff'') => (id'', inr ex, eff'')
-                              end
-                          | (id', inr ex, eff') => (id', inr ex, eff')
-                          end
-               end
-               ) env id l eff
-       in
-       match res with
-       | (id', inl vl, eff') => (id', inl (VTuple vl), eff')
-       | (id', inr ex, eff') => (id', inr ex, eff')
-       end
- | ECall f l => let res := 
-           (fix eval_list env id exps eff : nat * ((list Value) + Exception) * SideEffectList := 
-               match exps with
-               | []    => (id, inl [], eff)
-               | x::xs => match eval_fbos_expr env id x eff with
-                          | (id', inl v , eff') => 
-                            let res := eval_list env id' xs eff' in
-                              match res with
-                              | (id'', inl xs', eff'') => (id'', inl (v::xs'), eff'')
-                              | (id'', inr ex , eff'') => (id'', inr ex, eff'')
-                              end
-                          | (id', inr ex, eff') => (id', inr ex, eff')
-                          end
-               end
-               ) env id l eff
-       in
-       match res with
-       | (id', inl vl, eff') => let (a, b) := eval f vl eff' in (id', a, b)
-       | (id', inr ex, eff') => (id', inr ex, eff')
-       end
- | EApp exp l =>
-    match eval_fbos_expr env id exp eff with
-    | (id', inr ex, eff') => (id', inr ex, eff')
-    | (id', inl v , eff') => let res :=
-      (fix eval_list env id exps eff : nat * ((list Value) + Exception) * SideEffectList := 
-               match exps with
-               | []    => (id, inl [], eff)
-               | x::xs => match eval_fbos_expr env id x eff with
-                          | (id', inl v , eff') => 
-                            let res := eval_list env id' xs eff' in
-                              match res with
-                              | (id'', inl xs', eff'') => (id'', inl (v::xs'), eff'')
-                              | (id'', inr ex , eff'') => (id'', inr ex, eff'')
-                              end
-                          | (id', inr ex, eff') => (id', inr ex, eff')
-                          end
-               end
-               ) env id' l eff'
-       in
-       match res with
-       | (id'', inl vl, eff'') =>
-         match v with
-         | VClos ref ext idcl varl body => if Nat.eqb (length vl) (length varl)
-                                            then (id'', inl v, eff'')
-                                            (* eval_fbos_expr (append_vars_to_env varl vl (get_env ref ext)) id'' body eff'' *)
-                                            else (id'', inr (badarity v), eff'')
-         | _                             => (id'', inr (badfun v), eff'')
-         end
-       | (id'', inr ex, eff'') => (id'', inr ex, eff'')
-       end
+(* I can't import stdlib implementation somehow *)
+Definition list_sum l := fold_right plus 0 l.
+
+Fixpoint exp_size (e : Expression) : nat :=
+match e with
+ | ENil => 1
+ | ELit l => 1
+ | EVar v => 1
+ | EFunId f => 1
+ | EFun vl e => 1
+ | ECons hd tl => 1 + exp_size hd + exp_size tl
+ | ETuple l => 1 + list_sum (map exp_size l)
+ | ECall f l => 1 + list_sum (map exp_size l)
+ | EApp exp l => 1 + list_sum (map exp_size l) + exp_size exp
+ | ECase e l => 1 + exp_size e + fold_right (fun '(a, b, c) r => r + exp_size b + exp_size c) 0 l
+ | ELet v e1 e2 => 1 + exp_size e1 + exp_size e2
+ | ELetRec f l b e => 1 + exp_size e
+ | ETry e1 v1 e2 vl2 e3 => 1 + exp_size e1 + exp_size e2 + exp_size e3
+end.
+
+Fixpoint eval_list (f: Environment -> nat -> Expression -> SideEffectList -> nat -> option (nat * (Value + Exception) * SideEffectList)) (env : Environment) (id : nat) (exps : list Expression) (eff : SideEffectList) (clock : nat) : option (nat * ((list Value) + Exception) * SideEffectList) := 
+ match exps with
+ | []    => Some (id, inl [], eff)
+ | x::xs => match f env id x eff clock with
+            | Some (id', inl v , eff') => 
+              let res := eval_list f env id' xs eff' clock in
+                match res with
+                | Some (id'', inl xs', eff'') => Some (id'', inl (v::xs'), eff'')
+                | r => r
+                end
+            | Some (id', inr ex, eff') => Some (id', inr ex, eff')
+            | None => None
+            end
  end
-(*  | ECase e l =>
-    match eval_fbos_expr env id e eff with
-    | (id', inr ex, eff') => (id', inr ex, eff')
-    | (id', inl v , eff') =>
-     (fix clause_eval l i' :=
-     let i := (length l) - i' in
-       match i' with
-       | 0 => (id', inr if_clause, eff')
-       | S i'' =>
-       (* TODO: side effects cannot be produced here *)
-         match match_clause v l i with
-         | Some (gg, bb, bindings) =>
-           match eval_fbos_expr (add_bindings bindings env) id' gg eff' with
-           | (id'', inl v, eff'') =>  match v with
-                                      | VLit (Atom "true"%string)  => 
-                                          if (Nat.eqb id'' id') (* TODO: SE lists equal *)
-                                          then eval_fbos_expr (add_bindings bindings env) id' bb eff'
-                                          else (* undef *) (id'', inr novar, eff'')
-                                      | VLit (Atom "false"%string) => clause_eval l i''
-                                      | _ => (* TODO: undef *) (id', inr novar, eff')
-                                      end
-           | _                         => (* TODO: undef *) (id', inr novar, eff')
-           end
-         | None              => clause_eval l i''
-         end
+ .
+
+
+
+
+Fixpoint eval_fbos_expr (env : Environment) (id : nat) (exp : Expression) (eff : SideEffectList)  (clock : nat) : 
+  option (nat * (Value + Exception) * SideEffectList) :=
+match clock with
+| 0 => None
+| S clock' =>
+   match exp with
+   | ENil => Some (id, inl VNil, eff)
+   | ELit l => Some (id, inl (VLit l), eff)
+   | EVar v => Some (id, get_value env (inl v), eff)
+   | EFunId f => Some (id, get_value env (inr f), eff)
+   | EFun vl e => Some (S id, inl (VClos env [] id vl e), eff)
+   | ECons hd tl =>
+     match eval_fbos_expr env id hd eff clock' with
+     | Some (id', inl hdv, eff') =>
+       match eval_fbos_expr env id' tl eff' clock' with
+       | Some (id'', inl tlv, eff'') => Some (id'', inl (VCons hdv tlv), eff'')
+       | r => r
        end
-     ) l (length l)
-  end *)
- | ECase e l => (0, inr novar, [])
- | ELet var e1 e2 => 
-    match eval_fbos_expr env id e1 eff with
-    | (id', inr ex, eff') => (id', inr ex, eff')
-    | (id', inl v , eff') => eval_fbos_expr (append_vars_to_env [var] [v] env) id' e2 eff'
-    end
- | ELetRec f l b e => eval_fbos_expr (append_funs_to_env [(f, (l, b))] env id) (S id) e eff
- | ETry e1 v1 e2 vl2 e3 =>
-    match eval_fbos_expr env id e1 eff with
-    | (id', inr ex, eff') => eval_fbos_expr (append_try_vars_to_env vl2 [exclass_to_value (fst (fst ex)); snd (fst ex); snd ex] env) id' e3 eff'
-    | (id', inl v , eff') => eval_fbos_expr (append_vars_to_env [v1] [v] env) id' e2 eff'
-    end
+     | r => r
+     end
+   | ETuple l => 
+   let res := 
+      (fix eval_list env id exps eff : option (nat * ((list Value) + Exception) * SideEffectList) := 
+                 match exps with
+                 | []    => Some (id, inl [], eff)
+                 | x::xs => match eval_fbos_expr env id x eff clock' with
+                            | Some (id', inl v , eff') => 
+                              let res := eval_list env id' xs eff' in
+                                match res with
+                                | Some (id'', inl xs', eff'') => Some (id'', inl (v::xs'), eff'')
+                                | r => r
+                                end
+                            | Some (id', inr ex, eff') => Some (id', inr ex, eff')
+                            | None => None
+                            end
+                 end
+                 ) env id l eff
+         in
+         match res with
+         | Some (id', inl vl, eff') => Some (id', inl (VTuple vl), eff')
+         | Some (id', inr ex, eff') => Some (id', inr ex, eff')
+         | None => None
+         end
+   | ECall f l => let res := 
+             (fix eval_list env id exps eff : option (nat * ((list Value) + Exception) * SideEffectList) := 
+                 match exps with
+                 | []    => Some (id, inl [], eff)
+                 | x::xs => match eval_fbos_expr env id x eff clock' with
+                            | Some (id', inl v , eff') => 
+                              let res := eval_list env id' xs eff' in
+                                match res with
+                                | Some (id'', inl xs', eff'') => Some (id'', inl (v::xs'), eff'')
+                                | r => r
+                                end
+                            | Some (id', inr ex, eff') => Some (id', inr ex, eff')
+                            | None => None
+                            end
+                 end
+                 ) env id l eff
+         in
+         match res with
+         | Some (id', inl vl, eff') => let (a, b) := eval f vl eff' in Some (id', a, b)
+         | Some (id', inr ex, eff') => Some (id', inr ex, eff')
+         | None => None
+         end
+   | EApp exp l =>
+      match eval_fbos_expr env id exp eff clock' with
+      | Some (id', inl v , eff') => let res :=
+        (fix eval_list env id exps eff : option (nat * ((list Value) + Exception) * SideEffectList) := 
+                 match exps with
+                 | []    => Some (id, inl [], eff)
+                 | x::xs => match eval_fbos_expr env id x eff clock' with
+                            | Some (id', inl v , eff') => 
+                              let res := eval_list env id' xs eff' in
+                                match res with
+                                | Some (id'', inl xs', eff'') => Some (id'', inl (v::xs'), eff'')
+                                | r => r
+                                end
+                            | Some (id', inr ex, eff') => Some (id', inr ex, eff')
+                            | None => None
+                            end
+                 end
+                 ) env id l eff
+         in
+         match res with
+         | Some (id'', inl vl, eff'') =>
+           match v with
+           | VClos ref ext idcl varl body => if Nat.eqb (length vl) (length varl)
+                                              then (* Some (id'', inl v, eff'') *)
+                                              eval_fbos_expr (append_vars_to_env varl vl (get_env ref ext)) id'' body eff'' (clock')
+                                              else Some (id'', inr (badarity v), eff'')
+           | _                             => Some (id'', inr (badfun v), eff'')
+           end
+         | Some (id'', inr ex, eff'') => Some (id'', inr ex, eff'')
+         | None => None
+         end
+   | r => r
+   end
+  (*  | ECase e l =>
+      match eval_fbos_expr env id e eff with
+      | (id', inr ex, eff') => (id', inr ex, eff')
+      | (id', inl v , eff') =>
+       (fix clause_eval l i' :=
+       let i := (length l) - i' in
+         match i' with
+         | 0 => (id', inr if_clause, eff')
+         | S i'' =>
+         (* TODO: side effects cannot be produced here *)
+           match match_clause v l i with
+           | Some (gg, bb, bindings) =>
+             match eval_fbos_expr (add_bindings bindings env) id' gg eff' with
+             | (id'', inl v, eff'') =>  match v with
+                                        | VLit (Atom "true"%string)  => 
+                                            if (Nat.eqb id'' id') (* TODO: SE lists equal *)
+                                            then eval_fbos_expr (add_bindings bindings env) id' bb eff'
+                                            else (* undef *) (id'', inr novar, eff'')
+                                        | VLit (Atom "false"%string) => clause_eval l i''
+                                        | _ => (* TODO: undef *) (id', inr novar, eff')
+                                        end
+             | _                         => (* TODO: undef *) (id', inr novar, eff')
+             end
+           | None              => clause_eval l i''
+           end
+         end
+       ) l (length l)
+    end *)
+   | ECase e l => Some (0, inr novar, [])
+   | ELet var e1 e2 => 
+      match eval_fbos_expr env id e1 eff clock' with
+      | Some (id', inl v , eff') => eval_fbos_expr (append_vars_to_env [var] [v] env) id' e2 eff' clock'
+      | r => r
+      end
+   | ELetRec f l b e => eval_fbos_expr (append_funs_to_env [(f, (l, b))] env id) (S id) e eff clock'
+   | ETry e1 v1 e2 vl2 e3 =>
+      match eval_fbos_expr env id e1 eff clock' with
+      | Some (id', inr ex, eff') => eval_fbos_expr (append_try_vars_to_env vl2 [exclass_to_value (fst (fst ex)); snd (fst ex); snd ex] env) id' e3 eff' clock'
+      | Some (id', inl v , eff') => eval_fbos_expr (append_vars_to_env [v1] [v] env) id' e2 eff' clock'
+      | None => None
+      end
+  end
 end
 .
 
 Example exp1 := ELet "X"%string (ELet "X"%string (ELit (Integer 5)) (EVar "X"%string)) (ELet "X"%string (ELet "X"%string (ELit (Integer 5)) (EVar "X"%string)) (ELet "X"%string (ELet "X"%string (ELit (Integer 5)) (EVar "X"%string)) (ELet "X"%string (ELet "X"%string (ELit (Integer 5)) (EVar "X"%string)) (ELet "X"%string (ELet "X"%string (ELit (Integer 5)) (EVar "X"%string)) (ELet "X"%string (ELet "X"%string (ELit (Integer 5)) (EVar "X"%string)) (ELet "X"%string (ELet "X"%string (ELit (Integer 5)) (EVar "X"%string)) (ELet "X"%string (ELet "X"%string (ELit (Integer 5)) (EVar "X"%string)) (ELet "X"%string (ELet "X"%string (ELit (Integer 5)) (EVar "X"%string)) ( ELet "X"%string (ELet "X"%string (ELit (Integer 5)) (EVar "X"%string)) (ELet "X"%string (ELet "X"%string (ELit (Integer 5)) (EVar "X"%string)) (ELet "X"%string (ELet "X"%string (ELit (Integer 5)) (EVar "X"%string)) (ELet "X"%string (ELet "X"%string (ELit (Integer 5)) (EVar "X"%string)) (ELet "X"%string (ELet "X"%string (ELit (Integer 5)) (EVar "X"%string)) (ELet "X"%string (ELet "X"%string (ELit (Integer 5)) (EVar "X"%string)) (ELet "X"%string (ELet "X"%string (ELit (Integer 5)) (EVar "X"%string)) (ELet "X"%string (ELet "X"%string (ELit (Integer 5)) (EVar "X"%string)) (ELet "X"%string (ELet "X"%string (ELit (Integer 5)) (EVar "X"%string)) ( ELet "X"%string (ELet "X"%string (ELit (Integer 5)) (EVar "X"%string)) (ELet "X"%string (ELet "X"%string (ELit (Integer 5)) (EVar "X"%string)) (ELet "X"%string (ELet "X"%string (ELit (Integer 5)) (EVar "X"%string)) (ELet "X"%string (ELet "X"%string (ELit (Integer 5)) (EVar "X"%string)) (ELet "X"%string (ELet "X"%string (ELit (Integer 5)) (EVar "X"%string)) (ELet "X"%string (ELet "X"%string (ELit (Integer 5)) (EVar "X"%string)) (ELet "X"%string (ELet "X"%string (ELit (Integer 5)) (EVar "X"%string)) (ELet "X"%string (ELet "X"%string (ELit (Integer 5)) (EVar "X"%string)) (ELet "X"%string (ELet "X"%string (ELit (Integer 5)) (EVar "X"%string)) ( ELet "X"%string (ELet "X"%string (ELit (Integer 5)) (EVar "X"%string)) (ELet "X"%string (ELet "X"%string (ELit (Integer 5)) (EVar "X"%string)) (ELet "X"%string (ELet "X"%string (ELit (Integer 5)) (EVar "X"%string)) (ELet "X"%string (ELet "X"%string (ELit (Integer 5)) (EVar "X"%string)) (ELet "X"%string (ELet "X"%string (ELit (Integer 5)) (EVar "X"%string)) (ELet "X"%string (ELet "X"%string (ELit (Integer 5)) (EVar "X"%string)) (ELet "X"%string (ELet "Y"%string (ELit (Integer 5)) (EVar "Y"%string)) (ELet "X"%string (ELet "X"%string (ELit (Integer 5)) (EVar "X"%string)) (ELet "X"%string (ELet "X"%string (ELit (Integer 5)) (EVar "X"%string)) (ECall "+"%string [EVar "X"%string; EVar "X"%string])))))))))))))))))))))))))))))))))))).
 
-Compute eval_fbos_expr [] 0 exp1 [].
+Compute eval_fbos_expr [] 0 exp1 [] 10000.
